1.1.(i)
$$
\frac{\partial y_{i}}{\partial \gamma} = \hat{x_{i}}\\
\frac{\partial y_{i}}{\partial \beta} = 1
$$
1.1.(ii)
$$
\frac{\partial y_{j}}{\partial x_{i}} =
\left\{ \begin{aligned}  
0,i \neq j \lor r_{j}<p\\ 1/(1-p), i = j \land r_{j} \geq p 
\end{aligned}\right.
$$
1.1.(iii)
$$
\frac{\partial g(z)_{j}}{\partial z_{i}} = 
\left\{ \begin{aligned}
\frac{e^{z_i}(\Sigma_{j=1}^{k}e^{z_j})-e^{2z_{i}}}{(\Sigma_{j=1}^{k}e^{z_j})^2}, i = j\\
-\frac{e^{z_i+z_j}}{(\Sigma_{j=1}^{k}e^{z_j})^2},i\neq j
\end{aligned}\right.
$$

1.2.(i)
$$
z_{FC_{1a}} = \theta_{1a}x + b_{1a}\\
a_{FC_{1a}} = ReLU(z_{FC_{1A}})\\
a_{DP_{1a}} = M \bigodot a_{FC_{1a}}\\
\hat y_{a} = a_{FC_{2a}} = \theta_{2a}a_{DP_{1a}} + b_{2a}\\
z_{FC_{1b}} = \theta_{1b}x + b_{1b}\\
a_{FC_{1b}} = ReLU(z_{FC_{1b}})\\
a_{BN_{1b}} = BN_{\gamma,\beta}(a_{FC_{1b}})\\
z_{FC_{2b}} = \theta_{2b}(a_{BN_{1b}} \bigoplus a_{FC_{2a}}) + b_{2b}\\
\hat y_{b} = a_{FC_{2b}} = Softmax(z_{FC_{2b}})\\
L(x,y_a,y_b;\theta) = \frac{1}{m}\Sigma^{m}_{i=1}[\frac{1}{2}||(\hat y_{ai} - y_{ai})||^{2}_{2} - \Sigma_{j=1}^{n_{yb}}y_{bi}^{j}log(\hat y_{bi}^{j})]
$$
1.2.(ii)
$$
\frac{\partial L}{\partial z_{FC_{2b}}} = \frac{1}{m}\Sigma_{i=1}^{m}(\hat y_b^{(i)} - y_b^{(i)}),得到残差\delta^{(FC_{2b})}\\
\frac{\partial L}{\partial \theta_{2b}} = \delta^{(FC_{2b})} (a_{BN_{1b}} \oplus \hat y_{a})^{T}
$$

$$
\frac{\partial L}{\partial a_{BN_{1b}}}=\delta^{(FC_{2b})}\theta_{2b}^{T},得到残差\delta^{(BN_{1b})} \tag\\
\frac{\partial L}{\partial \gamma} = \delta^{(BN_{1b})}\hat a_{FC_{1b}}^{T}\\
\frac{\partial L}{\partial \beta}=\Sigma_{i=1}^{n_{ya}}\delta^{(BN_{1b})}_{i}\\
对于BN层，记输出a_{BN_{1b}}为y，记输入a_{FC_{1b}}为x，则有\\
\frac{\partial y_j}{\partial x_i} = 
\left\{ \begin{aligned}
\gamma (\sigma_{b}^{2}+\epsilon)^{-3/2}((1- \frac{1}{m})(\sigma_{b}^{2}+\epsilon) - \frac{1}{m}(x_j-\sigma_B)(x_i-\sigma_B),i = j\\
\gamma (\sigma_{b}^{2}+\epsilon)^{-3/2}(-\frac{1}{m}(\sigma_{b}^{2}+\epsilon) - \frac{1}{2}(x_j-\sigma_B)(x_i-\sigma_B),i \neq j
\end{aligned}\right.\\
\frac{\partial L}{\partial a_{FC_{1b}i}} = \Sigma_{j=1}^{m}\delta^{(BN_{1b})}\frac{\partial y_j}{\partial x_i}\\
$$

$$
\frac{\partial a_{FC_{1b}i}}{\partial z_{FC_{1b}i}}=sgn(z_{FC_{1b}i})\\
\frac{\partial L}{\partial z_{FC_{1b}i}}=\Sigma_{j=1}^{m}\delta^{(BN_{1b})}\frac{\partial y_j}{\partial x_i} \bigodot sgn(z_{FC_{1b}i}),记为残差\delta^{(FC_{1b})}\\
\frac{\partial L}{\partial \theta_{1b}}=\delta^{(FC_{1b})}x^{T}
$$


$$
\frac{\partial L}{\partial \hat y_{a}}= \frac{1}{m}\sum_{i=1}^{m}(\hat y_a^{(i)} - y_a^{(i)})+\delta^{(FC_{2b})}\theta_{2b}^{T},组合得到残差\delta^{(ya)}\\
\frac{\partial L}{\partial\theta_{2a}} = \delta^{(ya)}a_{DP_{1a}}^{T}\\
\frac{\partial L}{\partial a_{DP_{1a}}} = \delta^{(ya)}\theta_{2a}^{T},组合得到残差\delta^{(dp)}\\
\frac{\partial L}{\partial a_{FC_{1a}}i}=
\left\{ \begin{aligned}  
0,r_{i}<p\\ 
\frac{1}{1-p}\delta^{(dp)}_{i},r_{i} \geq p 
\end{aligned}\right. \\
\frac{\partial L}{\partial z_{FC_{1a}}i}=\frac{\partial L}{\partial a_{FC_{1a}}i}*Relu'(z_{FC_{1a}i})=\left\{ \begin{aligned}  
0,r_{i}<p\\ 
\frac{1}{1-p}\delta^{(dp)}_{i}sgn(z_{FC_{1a}i}),r_{i} \geq p 
\end{aligned}\right.,组合得到残差\delta^{(FC_{1a})}\\
\frac{\partial L}{\partial\theta_{1a}}=\delta^{(FC_{1a})}x^{T}\\
$$

